Examples/IMP.lean
@@ -1,6 +1,7 @@
 import Examples.IMP.Syntax
 import Examples.IMP.Semantics.Defs
 import Examples.IMP.Semantics.Lemmas
+import Examples.IMP.Abstraction
 import Examples.IMP.LTS
 import Examples.IMP.Programs.Assign
 import Examples.IMP.Programs.Branch
