Examples/IMP/Abstraction.lean
@@ -1,0 +1,2 @@
+import Examples.IMP.Abstraction.Defs
+import Examples.IMP.Abstraction.Lemmas
